theories/MaxOfTwoNumbers/Computed/AllLogits.v
@@ -1,0 +1,23 @@
+From NeuralNetInterp.MaxOfTwoNumbers Require Import Model.
+From NeuralNetInterp.Torch Require Import Tensor.
+From NeuralNetInterp.Util Require Import Pointed ValueExtraction.
+
+Local Notation prea := (logits all_tokens) (only parsing).
+Local Notation prev := (PArray.concretize prea) (only parsing).
+Local Definition pre := prev.
+
+Set NativeCompute Timing.
+(*Set NativeCompute Profiling.*)
+(* expected: about 45 minutes in vm, about 19 minutes in native *)
+Time Local Definition all_tokens_logits_concrete_value := native_compute pre.
+
+Time Definition all_tokens_logits_concrete : PArray.concrete_tensor _ _ := Eval hnf in extract all_tokens_logits_concrete_value.
+Definition all_tokens_logits_concrete_eq : all_tokens_logits_concrete = prev := extract_eq all_tokens_logits_concrete_value.
+
+Definition all_tokens_logits : tensor _ _ := PArray.reabstract (fun _ => prea) all_tokens_logits_concrete.
+Lemma all_tokens_logits_eq idxs : all_tokens_logits idxs = prea idxs.
+Proof.
+  cbv [all_tokens_logits].
+  erewrite PArray.reabstract_ext_correct by exact all_tokens_logits_concrete_eq.
+  reflexivity.
+Qed.
