theories/TransformerLens/HookedTransformer.v
@@ -1,0 +1,340 @@
+From Coq Require Import Floats Sint63 Uint63 QArith Lia List PArray Morphisms RelationClasses.
+From NeuralNetInterp.Util Require Import Default Pointed PArray List Notations Arith.Classes Arith.Instances Bool.
+From NeuralNetInterp.Util Require Nat Wf_Uint63.
+From NeuralNetInterp.Torch Require Import Tensor Einsum Slicing.
+Import Util.Nat.Notations.
+Import Util.Wf_Uint63.LoopNotation.
+Import Util.Wf_Uint63.
+Import Util.Wf_Uint63.Reduction.
+Import Arith.Instances.Truncating.
+Local Open Scope float_scope.
+Local Open Scope list_scope.
+Set Implicit Arguments.
+Import ListNotations.
+Local Open Scope raw_tensor_scope.
+
+(** Coq infra *)
+#[local] Coercion Uint63.of_Z : Z >-> Uint63.int.
+
+Notation tensor_of_list ls := (Tensor.PArray.abstract (Tensor.PArray.concretize (Tensor.of_list ls))) (only parsing).
+
+(*#[local] Notation FLOAT := float (only parsing). (* or Q *)*)
+
+Module Embed.
+  Section __.
+    Context {A d_vocab d_model}
+      (W_E : tensor A [d_vocab; d_model]).
+
+    Definition forward {r} {s : Shape r} (tokens : tensor IndexType s) : tensor A (s ::' d_model)
+      := (W_E.[tokens, :])%fancy_raw_tensor.
+  End __.
+End Embed.
+
+Module Unembed.
+  Section __.
+    Context {A} {addA : has_add A} {mulA : has_mul A} {zeroA : has_zero A}
+      {d_model d_vocab_out}
+      (W_U : tensor A [d_model; d_vocab_out])
+      (b_U : tensor A [d_vocab_out]).
+
+    Definition forward {r} {batch_pos : Shape r} (residual : tensor A (batch_pos ::' d_model))
+      : tensor A (batch_pos ::' d_vocab_out)
+      := (Tensor.map'
+            (fun residual : tensor A [d_model]
+             => weaksauce_einsum {{{ {{ d_model, d_model vocab -> vocab }}
+                        , residual
+                        , W_U }}}
+               : tensor A [d_vocab_out])
+            residual
+          + broadcast b_U)%core.
+  End __.
+End Unembed.
+
+Module PosEmbed.
+  Section __.
+    Context {A d_model}
+      {n_ctx:N}
+      (n_ctx' : int := n_ctx)
+      (W_pos : tensor A [n_ctx'; d_model]).
+
+    Definition forward {r} {batch : Shape r} {tokens_length} (tokens : tensor IndexType (batch ::' tokens_length))
+      : tensor A (batch ::' tokens_length ::' d_model)
+      := repeat (W_pos.[:tokens_length, :]) batch.
+  End __.
+End PosEmbed.
+
+Module LayerNorm.
+  Section __.
+    Context {r A} {s : Shape r} {d_model}
+      {addA : has_add A} {subA : has_sub A} {mulA : has_mul A} {divA : has_div A} {sqrtA : has_sqrt A} {zeroA : has_zero A} {coerZ : has_coer Z A} {default : pointed A}
+      (eps : A) (w b : tensor A [d_model]).
+
+    Definition linpart (x : tensor A (s ::' d_model))
+      : tensor A (s ::' d_model)
+      := (x - reduce_axis_m1 (keepdim:=true) mean x)%core.
+
+    Definition scale (x : tensor A (s ::' d_model))
+      : tensor A (s ::' 1)
+      := (√(reduce_axis_m1 (keepdim:=true) mean (x ²) + broadcast' eps))%core.
+
+    Definition rescale (x : tensor A (s ::' d_model))
+      (scale : tensor A (s ::' 1))
+      : tensor A (s ::' d_model)
+      := (x / scale)%core.
+
+    Definition postrescale (x : tensor A (s ::' d_model))
+      : tensor A (s ::' d_model)
+      := (x * broadcast w + broadcast b)%core.
+
+    Definition forward (x : tensor A (s ::' d_model))
+      : tensor A (s ::' d_model)
+      := let x := PArray.checkpoint (linpart x) in
+         let scale := scale x in
+         let x := rescale x scale in
+         PArray.checkpoint (postrescale x).
+  End __.
+End LayerNorm.
+
+Module Attention.
+  Section __.
+    Context {A r} {batch : Shape r}
+      {sqrtA : has_sqrt A} {coerZ : has_coer Z A} {addA : has_add A} {zeroA : has_zero A} {mulA : has_mul A} {divA : has_div A} {expA : has_exp A} {defaultA : pointed A}
+      {pos n_heads d_model d_head} {n_ctx:N}
+      {use_split_qkv_input : with_default "use_split_qkv_input" bool false}
+      (W_Q W_K W_V W_O : tensor A [n_heads; d_model; d_head])
+      (b_Q b_K b_V : tensor A [n_heads; d_head])
+      (b_O : tensor A [d_model])
+      (IGNORE : A := coerZ (-1 * 10 ^ 5)%Z)
+      (attn_scale : A := √(coer (Uint63.to_Z d_head)))
+      (maybe_n_heads := fun b : bool => (if b return Shape (if b then _ else _) then [n_heads] else [])%shape)
+      (query_input key_input value_input : tensor A ((batch ::' pos) ++' (maybe_n_heads use_split_qkv_input ::' d_model)))
+      (mask : tensor bool [n_ctx; n_ctx] := to_bool (tril (A:=bool) (ones [n_ctx; n_ctx]))).
+
+    (*         if self.cfg.use_split_qkv_input:
+            qkv_einops_string = "batch pos head_index d_model"
+        else:
+            qkv_einops_string = "batch pos d_model"
+
+        q = self.hook_q(
+            einsum(
+                f"{qkv_einops_string}, head_index d_model d_head \
+                -> batch pos head_index d_head",
+                query_input,
+                self.W_Q,
+            )
+            + self.b_Q
+        )  # [batch, pos, head_index, d_head]*)
+    Definition einsum_input
+      (input : tensor A ((batch ::' pos) ++' (maybe_n_heads use_split_qkv_input ::' d_model)))
+      (W : tensor A [n_heads; d_model; d_head])
+      : tensor A ((batch ::' pos) ++' [n_heads; d_head])
+      := Tensor.map'
+           (if use_split_qkv_input return tensor A (maybe_n_heads use_split_qkv_input ::' d_model) -> tensor A [n_heads; d_head]
+            then fun input => weaksauce_einsum {{{ {{ head_index d_model,
+                                          head_index d_model d_head
+                                          -> head_index d_head }}
+                                      , input
+                                      , W }}}
+            else fun input => weaksauce_einsum {{{ {{ d_model,
+                                          head_index d_model d_head
+                                          -> head_index d_head }}
+                                      , input
+                                      , W }}})
+           input.
+
+    Definition q : tensor A (batch ++' [pos; n_heads; d_head])
+      := PArray.checkpoint (einsum_input query_input W_Q + broadcast b_Q)%core.
+    Definition k : tensor A (batch ++' [pos; n_heads; d_head])
+      := PArray.checkpoint (einsum_input key_input W_K + broadcast b_K)%core.
+    Definition v : tensor A (batch ++' [pos; n_heads; d_head])
+      := PArray.checkpoint (einsum_input value_input W_V + broadcast b_V)%core.
+
+    Definition attn_scores : tensor A (batch ::' n_heads ::' pos ::' pos)
+      := (let qk : tensor A (batch ++' [n_heads; pos; pos])
+            := Tensor.map2'
+                 (fun q k : tensor A [pos; n_heads; d_head]
+                  => weaksauce_einsum
+                       {{{ {{ query_pos head_index d_head ,
+                                 key_pos head_index d_head
+                                 -> head_index query_pos key_pos }}
+                             , q
+                             , k }}}
+                    : tensor A [n_heads; pos; pos])
+                 q
+                 k in
+          PArray.checkpoint (qk / broadcast' attn_scale))%core.
+
+    Definition apply_causal_mask (attn_scores : tensor A (batch ::' n_heads ::' pos ::' pos))
+      : tensor A (batch ::' n_heads ::' pos ::' pos)
+      := Tensor.map'
+           (fun attn_scores : tensor A [pos; pos]
+            => Tensor.where_ mask.[:pos,:pos] attn_scores (broadcast' IGNORE))
+           attn_scores.
+
+    Definition masked_attn_scores : tensor A (batch ::' n_heads ::' pos ::' pos)
+      := apply_causal_mask attn_scores.
+
+    Definition pattern : tensor A (batch ::' n_heads ::' pos ::' pos)
+      := PArray.checkpoint (softmax_dim_m1 masked_attn_scores).
+
+    Definition z : tensor A (batch ::' pos ::' n_heads ::' d_head)
+      := PArray.checkpoint
+           (Tensor.map2'
+              (fun (v : tensor A [pos; n_heads; d_head])
+                   (pattern : tensor A [n_heads; pos; pos])
+               => weaksauce_einsum {{{ {{  key_pos head_index d_head,
+                              head_index query_pos key_pos ->
+                              query_pos head_index d_head }}
+                          , v
+                          , pattern }}}
+                 : tensor A [pos; n_heads; d_head])
+              v
+              pattern).
+
+    Definition attn_out : tensor A (batch ::' pos ::' d_model)
+      := (let out
+            := Tensor.map'
+                 (fun z : tensor A [pos; n_heads; d_head]
+                  => weaksauce_einsum {{{ {{ pos head_index d_head,
+                                 head_index d_head d_model ->
+                                 pos d_model }}
+                             , z
+                             , W_O }}}
+                    : tensor A [pos; d_model])
+                 z in
+          PArray.checkpoint (out + broadcast b_O))%core.
+  End __.
+End Attention.
+
+Module TransformerBlock.
+  Section __.
+    Context {A r} {batch : Shape r}
+      {zeroA : has_zero A} {coerZ : has_coer Z A}
+      {addA : has_add A} {subA : has_sub A} {mulA : has_mul A} {divA : has_div A}
+      {sqrtA : has_sqrt A} {expA : has_exp A}
+      {default : pointed A}
+      {pos n_heads d_model d_head} {n_ctx:N}
+      {use_split_qkv_input : with_default "use_split_qkv_input" bool false}
+      (W_Q W_K W_V W_O : tensor A [n_heads; d_model; d_head])
+      (b_Q b_K b_V : tensor A [n_heads; d_head])
+      (b_O : tensor A [d_model])
+      (eps : A)
+      (ln1_w ln1_b ln2_w ln2_b : tensor A [d_model])
+      (resid_pre : tensor A ((batch ::' pos) ++' [d_model]))
+      (maybe_n_heads := fun b : bool => (if b return Shape (if b then _ else _) then [n_heads] else [])%shape).
+
+    Definition add_head_dimension
+      (resid_pre : tensor A ((batch ::' pos) ++' [d_model]))
+      : tensor A ((batch ::' pos) ++' (maybe_n_heads use_split_qkv_input ::' d_model))
+      := if use_split_qkv_input return tensor A ((batch ::' pos) ++' (maybe_n_heads use_split_qkv_input ::' d_model))
+         then Tensor.map'
+                (fun resid_pre : tensor A [d_model]
+                 => Tensor.repeat resid_pre [n_heads]
+                   : tensor A [n_heads; d_model])
+                resid_pre
+         else resid_pre.
+    Definition query_input : tensor A ((batch ::' pos) ++' (maybe_n_heads use_split_qkv_input ::' d_model))
+      := add_head_dimension resid_pre.
+    Definition key_input : tensor A ((batch ::' pos) ++' (maybe_n_heads use_split_qkv_input ::' d_model))
+      := add_head_dimension resid_pre.
+    Definition value_input : tensor A ((batch ::' pos) ++' (maybe_n_heads use_split_qkv_input ::' d_model))
+      := add_head_dimension resid_pre.
+
+    Definition ln1 {r} {s : Shape r} (t : tensor A (s ::' d_model)) : tensor A (s ::' d_model)
+      := LayerNorm.forward eps ln1_w ln1_b t.
+    Definition ln2 {r} {s : Shape r} (t : tensor A (s ::' d_model)) : tensor A (s ::' d_model)
+      := LayerNorm.forward eps ln2_w ln2_b t.
+
+    Definition attn_only_out : tensor A (batch ++ [pos; d_model])
+      := (let attn_out : tensor A (batch ++ [pos; d_model])
+            := Attention.attn_out
+                 (n_ctx:=n_ctx)
+                 W_Q W_K W_V W_O
+                 b_Q b_K b_V b_O
+                 (ln1 query_input)
+                 (ln1 key_input)
+                 (ln1 value_input) in
+          resid_pre + attn_out)%core.
+  End __.
+End TransformerBlock.
+
+Module HookedTransformer.
+  Section __.
+    Context {A}
+      {zeroA : has_zero A} {coerZ : has_coer Z A}
+      {addA : has_add A} {subA : has_sub A} {mulA : has_mul A} {divA : has_div A}
+      {sqrtA : has_sqrt A} {expA : has_exp A}
+      {default : pointed A}
+      {d_vocab d_vocab_out n_heads d_model d_head} {n_ctx:N}
+      (*{use_split_qkv_input : with_default "use_split_qkv_input" bool false}*)
+      (eps : A)
+
+      (W_E : tensor A [d_vocab; d_model])
+      (W_pos : tensor A [n_ctx; d_model])
+
+      (blocks_params
+        : list ((* (W_Q W_K W_V W_O : tensor A [n_heads; d_model; d_head])
+      (b_Q b_K b_V : tensor A [n_heads; d_head])
+      (b_O : tensor A [d_model])
+      (ln1_w ln1_b : tensor A [d_model]) *)
+              tensor A [n_heads; d_model; d_head] * tensor A [n_heads; d_model; d_head] * tensor A [n_heads; d_model; d_head] * tensor A [n_heads; d_model; d_head]
+              * tensor A [n_heads; d_head] * tensor A [n_heads; d_head] * tensor A [n_heads; d_head]
+              * tensor A [d_model]
+              * tensor A [d_model] * tensor A [d_model]))
+
+      (ln_final_w ln_final_b : tensor A [d_model])
+
+      (W_U : tensor A [d_model; d_vocab_out]) (b_U : tensor A [d_vocab_out])
+    .
+
+    Section with_batch.
+      Context {r} {batch : Shape r} {pos}
+        (s := (batch ::' pos)%shape)
+        (resid_shape := (s ::' d_model)%shape).
+
+      Definition embed (tokens : tensor IndexType s) : tensor A resid_shape
+        := Embed.forward W_E tokens.
+
+      Definition pos_embed (tokens : tensor IndexType s) : tensor A resid_shape
+        := PosEmbed.forward W_pos tokens.
+
+      Definition blocks : list (tensor A resid_shape -> tensor A resid_shape)
+        := List.map
+             (fun '(W_Q, W_K, W_V, W_O,
+                    b_Q, b_K, b_V,
+                    b_O,
+                    ln1_w, ln1_b)
+              => TransformerBlock.attn_only_out
+                   (n_ctx:=n_ctx)
+                   W_Q W_K W_V W_O
+                   b_Q b_K b_V
+                   b_O
+                   eps
+                   ln1_w ln1_b)
+             blocks_params.
+
+      Definition ln_final (resid : tensor A resid_shape) : tensor A resid_shape
+        := LayerNorm.forward eps ln_final_w ln_final_b resid.
+
+      Definition unembed (resid : tensor A resid_shape) : tensor A (s ::' d_vocab_out)
+        := Unembed.forward W_U b_U resid.
+
+      Definition logits (tokens : tensor IndexType s) : tensor A (s ::' d_vocab_out)
+        := (let embed          := embed tokens in
+            let pos_embed      := pos_embed tokens in
+            let residual       := PArray.checkpoint (embed + pos_embed)%core in
+            (fun f ls a => List.fold_right f a ls residual)
+              (fun block cont residual
+               => let residual := PArray.checkpoint (block residual) in
+                  cont residual)
+              blocks
+              (fun residual
+               => let residual := PArray.checkpoint (ln_final residual) in
+                  let logits   := PArray.checkpoint (unembed residual) in
+                  logits)).
+
+      Definition forward (tokens : tensor IndexType s) : tensor A (s ::' d_vocab_out)
+        := logits tokens.
+    End with_batch.
+  End __.
+End HookedTransformer.
